added context to storage solvers

context.v
@@ -70,6 +70,9 @@ Definition chk_lt_wrt_ctx (ctx: ctx_t) (sv1 sv2: sstack_val) :=
   | _, _ => false
   end.
 
+Definition chk_neq_wrt_ctx (ctx: ctx_t) (sv1 sv2: sstack_val) :=
+  chk_lt_wrt_ctx ctx sv1 sv2 ||   chk_lt_wrt_ctx ctx sv2 sv1.
+
 
 End Context.
 
