context_facts.v
@@ -156,8 +156,7 @@ Qed.
 
 
 
-  
-
+    
   Lemma chk_lt_wrt_ctx_snd:
     forall ctx sv1 sv2,
       chk_lt_wrt_ctx ctx sv1 sv2 = true ->
@@ -167,7 +166,6 @@ Qed.
           eval_sstack_val sv1 model mem strg exts maxidx sb ops = Some v1 /\
             eval_sstack_val sv2 model mem strg exts maxidx sb ops = Some v2 /\
             wlt v1 v2.
-  Proof.
     intros ctx sv1 sv2 H_chkr model mem strg exts maxidx sb ops H_is_model.
     destruct ctx as [cs [chkr H_chkr_snd]].
     simpl in H_is_model.
@@ -301,4 +299,44 @@ Qed.
       apply H_chkr_snd.
 Qed.
 
+  Lemma chk_newq_wrt_ctx_snd:
+    forall ctx sv1 sv2,
+      chk_neq_wrt_ctx ctx sv1 sv2 = true ->
+      forall model mem strg exts maxidx sb ops,
+        is_model (ctx_cs ctx) model = true ->
+        exists v1 v2,
+          eval_sstack_val sv1 model mem strg exts maxidx sb ops = Some v1 /\
+            eval_sstack_val sv2 model mem strg exts maxidx sb ops = Some v2 /\
+            weqb v1 v2 = false.
+  Proof.
+    intros ctx sv1 sv2 H_imp_chkr model mem strg exts maxidx sb ops H_is_model.
+    unfold chk_neq_wrt_ctx in H_imp_chkr.
+    apply Bool.orb_true_iff in H_imp_chkr.
+    destruct H_imp_chkr as [H_imp_chkr | H_imp_chkr].
+    + pose proof (chk_lt_wrt_ctx_snd ctx sv1 sv2 H_imp_chkr model mem strg exts maxidx sb ops H_is_model) as H_chk_lt_wrt_ctx_snd.
+      destruct H_chk_lt_wrt_ctx_snd as [v1' [v2' [ H_eval_sv1 [H_eval_sv2 H_wlt_v1'_v2']]]].
+      exists v1'.
+      exists v2'.
+      rewrite H_eval_sv1.
+      rewrite H_eval_sv2.
+      repeat split; try reflexivity.
+      apply weqb_ne.
+      intuition.
+      rewrite H in H_wlt_v1'_v2'.
+      unfold wlt in H_wlt_v1'_v2'.
+      intuition.
+    + pose proof (chk_lt_wrt_ctx_snd ctx sv2 sv1 H_imp_chkr model mem strg exts maxidx sb ops H_is_model) as H_chk_lt_wrt_ctx_snd.
+      destruct H_chk_lt_wrt_ctx_snd as [v2' [v1' [ H_eval_sv2 [H_eval_sv1 H_wlt_v2'_v1']]]].
+      exists v1'.
+      exists v2'.
+      rewrite H_eval_sv1.
+      rewrite H_eval_sv2.
+      repeat split; try reflexivity.
+      apply weqb_ne.
+      intuition.
+      rewrite H in H_wlt_v2'_v1'.
+      unfold wlt in H_wlt_v2'_v1'.
+      intuition.
+Qed.
+  
 End ContextFacts.
