storage_ops_solvers_impl_soundness.v
@@ -62,6 +62,9 @@ Import Constraints.
 Require Import FORVES2.context.
 Import Context.
 
+Require Import FORVES2.context_facts.
+Import ContextFacts.
+
 Module StorageOpsSolversImplSoundness.
 
   Lemma trivial_sload_solver_snd: sload_solver_ext_snd trivial_sload_solver.
@@ -143,17 +146,23 @@ Module StorageOpsSolversImplSoundness.
           eval_sstack_val' (S maxidx) skey' model mem strg exts maxidx sbindings ops = Some v2 /\
           weqb v1 v2 = false.
   Proof.
+
+    Ltac ctx_tac ctx skey skey' H_neq model mem strg exts maxidx sbindings ops H_is_model :=
+      intros model mem strg exts H_is_model;
+      pose proof (chk_newq_wrt_ctx_snd ctx skey skey' H_neq model mem strg exts maxidx sbindings ops H_is_model) as H;
+      apply H.
+
     intros ctx skey skey' maxidx sbindings ops.
     intros H_valid_bs H_valid_skey H_valid_skey' H_neq.
     unfold not_eq_keys in H_neq.
-    destruct (follow_in_smap skey maxidx sbindings) as [skey_m|] eqn:E_follow_skey; try discriminate.
-    destruct skey_m; try discriminate.
-    destruct smv; try discriminate.
-    destruct val; try discriminate.
-    destruct (follow_in_smap skey' maxidx sbindings) as [skey'_m|] eqn:E_follow_skey'; try discriminate.
-    destruct skey'_m; try discriminate.
-    destruct smv; try discriminate.
-    destruct val0; try discriminate.
+    destruct (follow_in_smap skey maxidx sbindings) as [skey_m|] eqn:E_follow_skey; try (ctx_tac ctx skey skey' H_neq model mem strg exts maxidx sbindings ops H_is_model).
+    destruct skey_m; try (ctx_tac ctx skey skey' H_neq model mem strg exts maxidx sbindings ops H_is_model).
+    destruct smv; try (ctx_tac ctx skey skey' H_neq model mem strg exts maxidx sbindings ops H_is_model).
+    destruct val; try (ctx_tac ctx skey skey' H_neq model mem strg exts maxidx sbindings ops H_is_model).
+    destruct (follow_in_smap skey' maxidx sbindings) as [skey'_m|] eqn:E_follow_skey'; try (ctx_tac ctx skey skey' H_neq model mem strg exts maxidx sbindings ops H_is_model).
+    destruct skey'_m; try (ctx_tac ctx skey skey' H_neq model mem strg exts maxidx sbindings ops H_is_model).
+    destruct smv; try (ctx_tac ctx skey skey' H_neq model mem strg exts maxidx sbindings ops H_is_model).
+    destruct val0; try (ctx_tac ctx skey skey' H_neq model mem strg exts maxidx sbindings ops H_is_model).
     intros model mem strg exts.
     intros H_is_model.
     unfold eval_sstack_val' at 1.
